VisualProof.lean
@@ -1,4 +1,6 @@
 import VisualProof.Rule.Soundness
 import VisualProof.Rule.Executable
 import VisualProof.Rule.Lambda
+import VisualProof.Rule.Soundness.Lambda
+import VisualProof.Rule.Executable.Lambda
 import VisualProof.Rule.Completeness
