VisualProof/Rule/Soundness/Lambda.lean
@@ -1,2 +1,4 @@
 import VisualProof.Rule.Soundness.Lambda.Spawn
 import VisualProof.Rule.Soundness.Lambda.TermLeaf
+import VisualProof.Rule.Soundness.Lambda.Conversion
+import VisualProof.Rule.Soundness.Lambda.FreeVariableIdentity
